theories/L/Complexity/Problems/TMGenericNPcompleteProblem.v
@@ -24,7 +24,7 @@ Qed.
 
 Instance term_tapeToList sig {H:registered sig}:
   computableTime' (@tapeToList sig) (fun t _ => (sizeOfTape t*29 + 26,tt)).  
-extract. solverec. all:repeat simpl_list;cbn -[plus mult]. all:solverec.
+extract. recRel_prettify2. all:repeat (simpl_list;cbn -[plus mult]). all:nia.
 Proof.
 Qed.
 
@@ -55,6 +55,191 @@ Proof.
   
   eapply computableTimeExt. exact H'.
   extract. solverec. 
+Qed.
+
+Fixpoint forallb_time {X} (fT:X -> nat) xs :=
+  match xs with
+    [] => 8
+  | x :: xs => fT x + forallb_time fT xs + 15
+  end.
+
+Lemma forallb_time_eq X f (l:list X):
+  forallb_time f l = sumn (map f l) + length l * 15 + 8.
+Proof.
+  induction l;cbn;nia.
+Qed.
+
+Lemma forallb_time_const X c (l:list X):
+  forallb_time (fun _ =>  c) l = length l * (c+15) + 8.
+Proof.
+  induction l;cbn;nia.
+Qed.
+
+Instance term_forallb X {HX:registered X}:
+  computableTime' (@forallb X) (fun f t__f => (1,fun l _ => (forallb_time (fun x => fst (t__f x tt)) l,tt))).
+Proof.
+  extract.
+  solverec.
+Qed.
+
+From Undecidability Require Import L.Functions.EqBool.
+
+Definition allSameEntry_helper {X Y} eqbX eqbY `{_:eqbClass (X:=X) eqbX} `{eqbClass (X:=Y) eqbY}
+  := fun x y '(x', y') => implb (eqbX x (x':X)) (eqbY y (y':Y)).
+
+Instance term_allSameEntry_helper {X Y} {HX:registered X} {HY:registered Y}
+         `{eqbCompT X (R:=HX)} `{eqbCompT Y (R:=HY)}
+  :
+    computableTime' (@allSameEntry_helper X Y _ _ _ _) (fun x _ => (1,fun y _ =>(1,fun xy _ => (eqbTime x (fst xy) + eqbTime y (snd xy) + 18,tt)))).
+Proof.
+  unfold allSameEntry_helper. unfold implb. extract. solverec.
+Qed.
+
+Instance term_allSameEntry X Y {HX:registered X} {HY:registered Y}
+         `{eqbCompT X (R:=HX)} `{eqbCompT Y (R:=HY)}:
+  computableTime' (@allSameEntry X Y _ _ _ _) (
+                    fun x _ => (1,
+                             fun y _ => (1,
+                                      fun f _ =>(
+                                          length f * (size (enc x)*c__eqbComp X + size (enc y)* c__eqbComp Y + 42) + 12,tt)))).
+
+Proof.
+  unfold allSameEntry.
+  change (fun (x : X) (y : Y) (f : list (X * Y)) => forallb (fun '(x', y') => implb (eqb0 x x') (eqb1 y y')) f)with
+      (fun (x : X) (y : Y) f => forallb (allSameEntry_helper x y)  f).
+  extract.
+  recRel_prettify2. 1-2:easy.
+  clear.
+  rename x1 into f.
+  
+  change 12 with (8+4) at 3. rewrite !Nat.add_assoc. eapply plus_le_compat_r.
+  
+  induction f as [ | [x' y'] f].
+  { easy. }
+  cbn - [plus mult] . unfold eqbTime. rewrite IHf.
+  nia.
+Qed.
+
+Instance term_isInjFinfuncTable X Y {HX:registered X} {HY:registered Y}
+         `{eqbCompT X (R:=HX)} `{eqbCompT Y (R:=HY)}:
+  computableTime' (@isInjFinfuncTable X Y _ _ _ _) (fun f _ => (length f * (size (enc f) * (c__eqbComp X + c__eqbComp Y + 5)) + 8,tt)).
+Proof.
+  unfold isInjFinfuncTable. cbn. extract.
+  solverec. subst.
+  cbn [length]. rewrite !size_list. cbn [map sumn]. rewrite !size_prod. cbn [fst snd]. nia.
+Qed.
+
+Definition isBoundRead sig := fun a : option nat => match a with
+                                               | Some a0 => a0 <? sig
+                                               | None => true
+                                               end.
+Definition isBoundWrite sig := (fun a : option nat * move => match fst a with
+                                                        | Some a0 => a0 <? sig
+                                                        | None => true
+                                                        end).
+Lemma size_option X {_:registered X} (o:option X) :
+  size (enc o)= match o with
+                  None => 3
+                | Some x => size (enc x) + 5
+                end.
+Proof.
+  change (enc o) with (LOptions.option_enc o).
+  destruct o.
+  all:cbn [LOptions.option_enc map sumn size].
+  all:solverec. 
+Qed.
+
+Instance term_isBoundRead:
+  computableTime' isBoundRead (fun sig _ => (1, fun s _ => (size (enc s) * 4,tt))).
+Proof.
+  unfold isBoundRead,Nat.ltb. extract. solverec.
+  
+  all:rewrite size_option.
+  all:try rewrite size_nat_enc. all:solverec. 
+Qed.
+
+Instance term_isBoundWrite:
+  computableTime' isBoundWrite (fun sig _ => (1, fun s _ => (size (enc s) * 4,tt))).
+Proof.
+  unfold isBoundWrite,Nat.ltb. extract.
+  recRel_prettify2.
+  all:try rewrite size_prod;cbn [fst snd] in *;subst;repeat rewrite size_option,!size_nat_enc. all:solverec. 
+Qed.
+
+Definition isBoundEntry sig n states: (nat * list (option nat) * (nat * list (option nat * move))) -> bool:= 
+  (fun '(s, v, (s', v')) =>
+     (s <? states)
+       && (| v | =? n)
+       && forallb (isBoundRead sig) v
+       && (s' <? states) && (| v' | =? n) &&
+       forallb (isBoundWrite sig) v').
+
+Lemma sumn_map_add X f g (l:list X) :
+  sumn (map (fun x => f x + g x) l) = sumn (map f l) + sumn (map g l).
+Proof.
+  induction l;cbn;nia.
+Qed.
+Lemma sumn_map_mult_c_r X f c (l:list X) :
+  sumn (map (fun x => f x *c) l) = sumn (map f l)*c.
+Proof.
+  induction l;cbn;nia.
+Qed.
+Lemma sumn_map_c X c (l:list X) :
+  sumn (map (fun _ => c) l) = length l * c.
+Proof.
+  induction l;cbn;nia.
+Qed.
+
+Instance term_isBoundEntry:
+  computableTime' isBoundEntry (fun sig _ => (1,
+                                           fun n _ => (1,
+                                                    fun states _ => (1,
+                                                                  fun e _ => 
+                                                                    (size (enc e)* (8+c__eqbComp nat),tt))))).
+Proof.
+  unfold isBoundEntry, Nat.ltb. extract. 
+  
+  recRel_prettify2. 1-3:nia. 
+  all:rewrite !size_prod;cbn [fst snd].
+  all:rewrite !forallb_time_eq. 
+  all:rewrite !size_list.
+  
+  
+  all:rewrite !sumn_map_add,!sumn_map_mult_c_r,!sumn_map_c.
+  all:unfold eqbTime.
+  all:rewrite !Nat.le_min_l.
+  all:rewrite !size_nat_enc. all:zify. all:clear; nia. 
+Qed.
+
+Instance term_isBoundTransTable:
+  computableTime' isBoundTransTable (fun _ _ => (1,
+                                              fun _ _ => (1,
+                                                       fun _ _ => (1,
+                                                                fun f _ => 
+                                                                  (size (enc f)* (8+c__eqbComp nat),tt))))).
+Proof.
+  unfold isBoundTransTable.
+  eapply computableTimeExt with (x:=fun sig n states f => forallb (isBoundEntry sig n states) f).
+  {reflexivity. }
+  extract.
+  solverec.
+  rewrite forallb_time_eq.
+  rewrite !size_list.
+  rewrite !sumn_map_mult_c_r.
+  rewrite !sumn_map_add, !sumn_map_c.
+  all:ring_simplify. zify. clear; nia.
+Qed.
+
+Instance term_isValidFlatTrans:
+  computableTime' (isValidFlatTrans) (fun _ _ => (1,
+                                               fun _ _ => (1,
+                                                        fun states_ _ => (1,
+                                                                       fun f _ => 
+                                                                         (size (enc f)* (8+c__eqbComp nat + length f * (c__eqbComp (nat*(list (option nat)))
+                                                                                                                    + c__eqbComp (nat*(list (option nat * move))) + 5))+ 17,tt))))).
+Proof.
+  unfold isInjFinfuncTable. cbn. extract.
+  solverec.
 Qed.
 
 Lemma inNP_TMgenericNPCompleteProblem:
@@ -115,15 +300,7 @@ Proof.
      }
      eexists.
 
-(*
-     Instance term_allSameEntry X Y {HX:registered X} {HY:registered Y}:
-       computableTime' (@allSameEntry X Y) (fun _ t__X => (1,fun _ t__Y => (1, fun x _ => (1, fun y _ => (1,fun f _ => (cnst 0,tt)))))).
-     Proof.
-       extract. *)
-     
-     Print allSameEntry.
-     Print isInjFinfuncTable.
-     Print isValidFlatTrans.
+     (* TODO: size flat TM *)
      Print isValidFlatTM.
      Fail now extract. all:admit. 
    }
