theories/L/Functions/Subst.v
@@ -1,8 +1,14 @@
-From Undecidability.L Require Import Tactics.LTactics Functions.Equality Datatypes.LNat.
+From Undecidability.L Require Import Tactics.LTactics Datatypes.LNat Functions.EqBool Datatypes.LTerm.
 (** ** Extracted substitution on terms *)
 
 Instance term_substT :
-  computableTime' subst (fun s _ => (5, (fun n _ => (1, (fun t _ => ( 15 * n * size s + 43 * (size s) ^ 2 + 13, tt)))))).
+  computableTime' subst (fun s _ => (5, (fun n _ => (1, (fun t _ => ( (* n * (cnst 0+15) * size s + *) (size s) * (size s + c__eqbComp nat * 4 + 20), tt)))))).
 Proof.
-  extract. solverec.
+  unfold subst. change Nat.eqb with (EqBool.eqb (X:=nat)).
+  extract.
+
+  recRel_prettify2. all:unfold eqbTime; cbn [fst snd size].
+  all:try rewrite !size_nat_enc.
+  all:try rewrite Nat.le_min_l.
+  all:ring_simplify. all:try nia.
 Qed.
